More work on CEK and clarifying list continuations

src/CEK.v
@@ -34,20 +34,28 @@ Equations get `(se : Env Γ) `(v : Var Γ τ) : Value τ :=
   get (Val x _)   ZV    := x;
   get (Val _ xs) (SV v) := get xs v.
 
+Inductive Accum Γ : ∀ τ : Ty, Exp Γ τ → Type :=
+  | ANone {τ e} : Accum Γ τ e
+  | AList {τ l} : list (Value τ) → Accum Γ (TyList τ) (List l).
+
+Arguments ANone {Γ τ e}.
+Arguments AList {Γ τ l} _.
+
+Derive Signature NoConfusion Subterm for Accum.
+
 Inductive Kont : Ty → Ty → Type :=
   | Mt {a} : Kont a a
   | Ar {Γ a b c} : Exp Γ a → Env Γ → Kont b c → Kont (a ⟶ b) c
-  | Nv {a b} : (Value a → Σ b) → Kont a b
+  | Fn {a b} : (Value a → Σ b) → Kont a b
 
 with Σ : Ty → Type :=
-  | MkΣ
-      (τ   : Ty)
-      (Γ   : Exp.Env)
-      (r   : Ty)
-      (exp : Exp Γ r)
-      (env : Env Γ)
-      (acc : option (Value r))
-      (knt : Kont r τ) : Σ τ.
+  | MkΣ (τ   : Ty)
+        (Γ   : Exp.Env)
+        (r   : Ty)
+        (exp : Exp Γ r)
+        (env : Env Γ)
+        (acc : Accum Γ r exp)
+        (knt : Kont r τ) : Σ τ.
 
 Derive Signature NoConfusion for Kont.
 Derive Signature NoConfusion Subterm for Σ.
@@ -57,52 +65,53 @@ Arguments MkΣ {τ Γ r} _ _ _.
 (* Inject the expression into a [Σ] whose final continuation will receive the
    results of the evaluation. Therefore, the resulting [env] will be a
    singleton list containing that value. *)
-Definition inject {τ : Ty} (e : Exp [] τ) : Σ τ := MkΣ e Empty None Mt.
+Definition inject {τ : Ty} {Γ : Exp.Env} (e : Exp Γ τ) (E : Env Γ) : Σ τ :=
+  MkΣ e E ANone Mt.
 
 Equations step {τ : Ty} (s : Σ τ) : Σ τ :=
   (* A constant is passed as a literal *)
-  step (MkΣ (Constant x) _ _ (Nv f)) :=
+  step (MkΣ (Constant x) _ ANone (Fn f)) :=
     f (VLit x);
 
   (* Lists are evaluated step-wise using Ls *)
-  step (MkΣ (List []) ρ None (Nv f)) :=
+  step (MkΣ (List []) ρ ANone (Fn f)) :=
     f (VList []);
-  step (MkΣ (List []) ρ (Some (VList r)) (Nv f)) :=
+  step (MkΣ (List []) ρ (AList r) (Fn f)) :=
     f (VList (rev r));
 
-  step (MkΣ (List (x :: xs)) ρ None κ) :=
-    MkΣ x ρ None (Nv (λ v, MkΣ (List xs) ρ (Some (VList [v])) κ));
-  step (MkΣ (List (x :: xs)) ρ (Some (VList r)) κ) :=
-    MkΣ x ρ None (Nv (λ v, MkΣ (List xs) ρ (Some (VList (v :: r))) κ));
+  step (MkΣ (List (x :: xs)) ρ ANone κ) :=
+    MkΣ x ρ ANone (Fn (λ v, MkΣ (List xs) ρ (AList [v]) κ));
+  step (MkΣ (List (x :: xs)) ρ (AList r) κ) :=
+    MkΣ x ρ ANone (Fn (λ v, MkΣ (List xs) ρ (AList (v :: r)) κ));
 
   (* A sequence just evaluates the second, for now *)
-  step (MkΣ (Seq e1 e2) ρ r κ) :=
-    MkΣ e2 ρ r κ;
+  step (MkΣ (Seq e1 e2) ρ ANone κ) :=
+    MkΣ e2 ρ ANone κ;
 
   (* Let is a simple desugaring *)
-  step (MkΣ (Let x body) ρ r κ) :=
-    MkΣ (APP (LAM body) x) ρ r κ;
+  step (MkΣ (Let x body) ρ ANone κ) :=
+    MkΣ (APP (LAM body) x) ρ ANone κ;
 
   (* A variable might lookup a lambda, in which case continue evaluating down
      that vein; otherwise, if no continuation, this is as far as we can go. *)
-  step (MkΣ (VAR v) ρ r κ) with get ρ v := {
-    | VClosure (Lambda e ρ') => MkΣ (LAM e) ρ' r κ
+  step (MkΣ (VAR v) ρ _ κ) with get ρ v := {
+    | VClosure (Lambda e ρ') => MkΣ (LAM e) ρ' ANone κ
     | x with κ := {
-        | Nv f => f x
-        | Mt => MkΣ (VAR v) ρ r Mt
+        | Fn f => f x
+        | Mt => MkΣ (VAR v) ρ ANone Mt
       }
   };
 
   (* Lambda evaluates its argument, with the lambda as the cont *)
-  step (MkΣ (LAM e) ρ r (Ar a ρ' κ)) :=
-    MkΣ a ρ' None (Nv (λ v, MkΣ e (Val v ρ) None κ));
+  step (MkΣ (LAM e) ρ ANone (Ar a ρ' κ)) :=
+    MkΣ a ρ' ANone (Fn (λ v, MkΣ e (Val v ρ) ANone κ));
   (* If a lambda is passed, call it with the continuation *)
-  step (MkΣ (LAM e) ρ _ (Nv f)) :=
+  step (MkΣ (LAM e) ρ ANone (Fn f)) :=
     f (VClosure (Lambda e ρ));
 
   (* Application evaluates the lambda and then the argument *)
-  step (MkΣ (APP e1 e2) ρ r κ) :=
-    MkΣ e1 ρ None (Ar e2 ρ κ);
+  step (MkΣ (APP e1 e2) ρ ANone κ) :=
+    MkΣ e1 ρ ANone (Ar e2 ρ κ);
 
   (* Otherwise, there is nothing more that can be done *)
   step (MkΣ s ρ r Mt) := MkΣ s ρ r Mt.
@@ -110,69 +119,83 @@ Equations step {τ : Ty} (s : Σ τ) : Σ τ :=
 Equations loop (gas : nat) {τ : Ty} (s : Σ τ) : Σ τ + Value τ :=
   loop O s :=
     inl s;
-  loop _ (MkΣ (Constant x) _ _ Mt) :=
+  loop _ (MkΣ (Constant x) _ ANone Mt) :=
     inr (VLit x);
-  loop _ (MkΣ (List []) _ None Mt) :=
+  loop _ (MkΣ (List []) _ ANone Mt) :=
     inr (VList []);
-  loop _ (MkΣ (List []) _ (Some (VList r)) Mt) :=
+  loop _ (MkΣ (List []) _ (AList r) Mt) :=
     inr (VList (rev r));
-  loop _ (MkΣ (VAR v) ρ _ Mt) :=
+  loop _ (MkΣ (VAR v) ρ ANone Mt) :=
     inr (get ρ v);
   loop (S gas') s :=
     loop gas' (step s).
 
-Definition run (gas : nat) {τ : Ty} (e : Exp [] τ) : Σ τ + Value τ :=
-  loop gas (inject e).
+Equations loop' (gas : nat) {τ : Ty} (s : Σ τ) : Σ τ :=
+  loop' O s := s;
+  loop' (S gas') s := loop' gas' (step s).
 
-Example constant_integer :
-  run 10 (Constant (LInteger 123%Z)) = inr (VLit (LInteger 123%Z)).
+Definition run (gas : nat) {τ : Ty} {Γ : Exp.Env} (e : Exp Γ τ) (E : Env Γ) :
+  Σ τ + Value τ := loop gas (inject e E).
+
+Example exp_constant :
+  run 10 (Constant (LInteger 123%Z)) Empty = inr (VLit (LInteger 123%Z)).
 Proof. reflexivity. Qed.
 
-Example constant_lam_integer :
-  run 10 (APP (LAM (VAR ZV)) (Constant (LInteger 123%Z))) =
-    inr (VLit (LInteger 123%Z)).
-Proof. reflexivity. Qed.
-
-Compute run 20 (List (Constant (LInteger 123%Z) ::
-                      Constant (LInteger 456%Z) ::
-                      Constant (LInteger 789%Z) :: [])).
-
-Example constant_cons :
+Example exp_list :
   run 20 (List (Constant (LInteger 123%Z) ::
                 Constant (LInteger 456%Z) ::
-                Constant (LInteger 789%Z) :: [])) =
+                Constant (LInteger 789%Z) :: [])) Empty =
     inr (VList (VLit (LInteger 123%Z) ::
                 VLit (LInteger 456%Z) ::
                 VLit (LInteger 789%Z) :: [])).
 Proof. reflexivity. Qed.
-(*
+
+Example exp_let :
+  run 10 (Let (Constant (LInteger 123%Z)) (VAR ZV)) Empty =
+    inr (VLit (LInteger 123%Z)).
+Proof. reflexivity. Qed.
+
+Example exp_var :
+  run 10 (VAR ZV) (Val (VLit (LInteger 123%Z)) Empty) =
+    inr (VLit (LInteger 123%Z)).
+Proof. reflexivity. Qed.
+
+Example exp_lam τ :
+  run 10 (LAM (cod:=τ) (VAR ZV)) Empty =
+    inl (MkΣ (LAM (VAR ZV)) Empty ANone Mt).
+Proof. reflexivity. Qed.
+
+Example exp_app :
+  run 10 (APP (LAM (VAR ZV)) (Constant (LInteger 123%Z))) Empty =
+    inr (VLit (LInteger 123%Z)).
+Proof. reflexivity. Qed.
+
 Theorem cek_sound τ (e : Exp [] τ) v :
-  Eval e v → ∃ gas, run gas e = MkΣ v Empty Mt.
+  Eval e v → ∃ gas, loop' gas (inject e Empty) = MkΣ v Empty ANone Mt.
 Proof.
   unfold run, Basics.compose, inject.
   intros.
   induction H; simpl; intros; auto.
   - exists 1%nat; simpl.
-    now rewrite step_equation_2.
+    rewrite loop'_equation_2.
+    now rewrite step_equation_1.
   - destruct IHEval as [gas' IHEval'].
     now exists (S gas').
+  - destruct IHEval as [gas' IHEval'].
+    exists (S gas'); simpl.
+    rewrite loop'_equation_2.
+    now rewrite step_equation_10.
   - exists 1%nat; simpl.
-    now rewrite step_equation_5.
-  - destruct IHEval1 as [gas1 IHEval1'].
-    destruct IHEval2 as [gas2 IHEval2'].
-    exists (S (S (S (gas1 + gas2)))).
-    rewrite step_equation_7.
-    admit.
+    rewrite loop'_equation_2.
+    rewrite step_equation_12.
+    now rewrite loop'_equation_1.
   - destruct IHEval1 as [gas1 IHEval1].
     destruct IHEval2 as [gas2 IHEval2].
-    exists (S (S (S (gas1 + gas2)))).
-    rewrite step_equation_8.
-    rewrite step_equation_13.
-    rewrite step_equation_11.
+    destruct IHEval3 as [gas3 IHEval3].
+    exists (S (S (S (gas1 + gas2 + gas3)))).
+    rewrite loop'_equation_2.
+    rewrite step_equation_15.
     admit.
-  - admit.
-  - admit.
 Abort.
-*)
 
 End CEK.
